theories/Monads/STMonad.v
@@ -1,81 +1,60 @@
 (* Copyright 2026 Bloomberg Finance L.P. *)
 (* Distributed under the terms of the GNU LGPL v2.1 license. *)
 
-From Crane Require Import Monads.ITree.
-From ExtLib Require Import
-  Structures.Maps
-  Structures.Functor
-  Data.Map.FMapAList
-.
-
-From ExtLib Require Import
-     Structures.Maps
-     Structures.Traversable
-     Data.Monads.EitherMonad
-     Data.List
-     Data.Pair
-     Data.Bool
-     Data.Map.FMapAList
-     Data.String
-.
-
-From ITree Require Import
-  ITree
-  ITreeFacts
-  Events.MapDefault
-  Events.MapDefaultFacts
-  Events.Exception
-  Events.FailFacts
-  Events.State
-  Eq.Paco2
-  Basics.HeterogeneousRelations
-  HasPost
-.
 From Stdlib Require Import
+  Arith.PeanoNat
+  Arith.Peano_dec
+  Init.Peano
   List
+  Morphisms
+  RelationClasses
+  Relation_Definitions
+  Setoid
   Strings.String
 .
 
-
-(* TODO: nit; organize imports *)
-From ITree Require Import
-  ITree
-  ITreeFacts
-  Events.MapDefault
-  Events.MapDefaultFacts
-  Events.Exception
-  Events.FailFacts
-  Events.State
+From Crane Require Import Monads.ITree Utils.HMap Utils.HAList Extraction.
+From ExtLib Require Import
+  Data.Bool
+  Data.List
+  Data.Monads.EitherMonad
+  Data.Pair
+  Data.String
+  Structures.Functor
+  Structures.Traversable
 .
 
+(* NOTE: *must* import this before the ITree Eq.Paco2 import.*)
 From Paco Require Import paco.
 
 From ITree Require Import
+  Basics.HeterogeneousRelations
+  Eq.Paco2
+  Events.Exception
+  Events.FailFacts
+  Events.MapDefault
+  Events.MapDefaultFacts
+  Events.State
+  Events.StateFacts
   ITree
   ITreeFacts
-  Events.StateFacts
-  Events.Exception
-  Events.State
-  Eq.Paco2
-  Basics.HeterogeneousRelations
-  HasPost
 .
 
 Import Monads.
 Import ListNotations.
-From Stdlib Require Import
-  Morphisms
-  Setoid
-  Relation_Definitions
-  RelationClasses
-  Arith.PeanoNat
-  Arith.Peano_dec
-  Init.Peano
-.
 Import ProperNotations.
 Local Open Scope monad_scope.
 Local Open Scope string_scope.
 
+
+(* Used for runtime checks, though an ideal impl won't need these. *)
+
+Variant Err : Type :=
+| Error (x : string) : Err.
+
+Definition failwith
+  {E : Type -> Type} `{exceptE Err -< E}
+  {A:Type} (s:string) : itree E A := throw (Error s).
 
 
 Module Type ST_SIG.
@@ -84,10 +63,21 @@ Module Type ST_SIG.
   Parameter STRef : forall S A : Type, Type. 
   Parameter IdxDecEq : forall (S : Type) (i1 i2 : Idx S),  
       {i1 = i2} + {i1 <> i2}.
-  (* TODO: can we tie the result index to the stref here? *)
   Parameter mkSTRef : forall S A : Type, Idx S -> STRef S A.
   Parameter STRefToIdx : forall (S A : Type), STRef S A -> Idx S. 
-
+  Parameter STEvent : forall S : Type, (Idx S -> Type) -> Type -> Type.
+  Parameter newSTRef : forall {E : Type -> Type} {S : Type}
+                         (V : (Idx S -> Type)) `{STEvent S V -< E}
+                         (I : Idx S),
+      V I -> itree E (STRef S (V I)).
+  Parameter readSTRef : forall {E : Type -> Type} {S : Type} 
+                        (V : Idx S -> Type) `{STEvent S V -< E}
+                        (I : Idx S),
+      STRef S (V I) -> itree E (V I).
+  Parameter writeSTRef : forall {E : Type -> Type} {S : Type} 
+                        (V : Idx S -> Type) `{STEvent S V -< E}
+                        (I : Idx S),
+      STRef S (V I) -> V I -> itree E unit.
 
   (* Used to generate fresh, unique indices.*)
   Parameter IdxGenE : Type -> Type.
@@ -100,8 +90,11 @@ Module Type ST_SIG.
   Parameter IdxRefSameIdx: forall (S A : Type) (idx : Idx S), (STRefToIdx S A (mkSTRef S A idx)) = idx.
   Parameter IdxRefSameRef: forall (S A : Type) (ref : STRef S A), (mkSTRef S A (STRefToIdx S A ref)) = ref.
 
+  (* TODO: indices are ordered. *)
+  (* TODO: indices are unique. *)
 
 End ST_SIG.
+
 
 Module ST_IMPL : ST_SIG.
 
@@ -140,225 +133,154 @@ Module ST_IMPL : ST_SIG.
   Proof. intros. cbn. unfold STRefToIdx. destruct ref. reflexivity. Qed.
   
 
-End ST_IMPL.
-
-Import ST_IMPL.
-
-(* TODO: Expand to cover more types than nat *)
-Variant STEvent (S : Type) : Type -> Type :=
-  | NewSTRef (v : nat) : STEvent S (STRef S nat)
-  | ReadSTRef : STRef S nat -> STEvent S nat
-  | WriteSTRef : STRef S nat -> nat -> STEvent S unit
-.
 
 
-(* Used for runtime checks, though an ideal impl won't need these. *)
+  Variant STEvent' (S : Type) {V : (Idx S) -> Type} : Type -> Type :=
+    | NewSTRef (I : Idx S) (v : V I) : STEvent' S (STRef S (V I))
+    | ReadSTRef (I : Idx S) : STRef S (V I) -> STEvent' S (V I)
+    | WriteSTRef (I : Idx S) : STRef S (V I) -> (V I) -> STEvent' S unit
+  .
 
-Variant Err : Type :=
-| Error (x : string) : Err.
+  Definition STEvent := STEvent'.
 
-Definition failwith
-  {E : Type -> Type} `{exceptE Err -< E}
-  {A:Type} (s:string) : itree E A := throw (Error s).
+
   
 
 Section Translation.
 
   Context {E : Type -> Type}.
   Context {S : Type}.
-  Context `{STEvent S -< E}. 
+  Context {V : (Idx S) -> Type}.
+  Context `{@STEvent S V -< E}. 
+  Context `{exceptE Err -< E}.
+  Context `{IdxGenE -< E}.
 
   
   Definition lookup_err
-    {E : Type -> Type} {R : Type}
-    `{exceptE Err -< E}
-    {map} `{Map (Idx S) R map}
-    (k : (Idx S)) (mem : map) : itree E R :=
+    {V : (Idx S) -> Type}
+    {map} `{HMap (Idx S) V map}
+    (k : (Idx S)) (mem : map) : itree E (V k) :=
     match lookup k mem with
       | None => throw (Error "Failed to find key in map")
       | Some v => Ret v
     end.
 
   
-  Definition newSTRef (v : nat) : itree E (STRef S nat) :=
-    trigger (NewSTRef S v). 
+  Definition newSTRef {I : Idx S} (v : (V I)) : itree E (STRef' S (V I)) :=
+    trigger (NewSTRef S I v). 
 
-  Definition readSTRef (ref : STRef S nat) : itree E nat :=
-    trigger (ReadSTRef S ref). 
+  Definition readSTRef {I : Idx S} (ref : STRef' S (V I)) : itree E (V I) :=
+    trigger (ReadSTRef S I ref).
 
-  Definition writeSTRef (ref : STRef S nat) (a : nat) : itree E unit :=
-    trigger (WriteSTRef S ref a).
+  Definition writeSTRef {I : Idx S} (ref : STRef' S (V I)) (a : (V I)) : itree E unit :=
+    trigger (WriteSTRef S I ref a).
 
 
+  (* TODO: cleanup! *)
   Definition handle_STEvent
-    {map} `{Map (Idx S) nat map}
-    `{IdxGenE -< E} `{exceptE Err -< E}
-    : forall (T : Type),  STEvent S T -> stateT map (itree E) T :=
+    {map} `{HMap (Idx S) V map}
+    : forall (T : Type), @STEvent S V T -> stateT map (itree E) T :=
     fun T e mem =>
-    match e in (STEvent _ T0) return (itree E (map * T0)) with
-    | NewSTRef _ v => idx <- newIdx;; Ret (add idx v mem, mkSTRef S nat idx)
-    | ReadSTRef _ s =>
-        let idx := STRefToIdx S nat s in v <- lookup_err idx mem;; Ret (mem, v)
-    | WriteSTRef _ s n => let idx := STRefToIdx S nat s in Ret (add idx n mem, tt)
-    end.
+      match e in (STEvent' _ T0) return (itree E (map * T0)) with
+      | NewSTRef _ Id v =>
+        idx <- @newIdx S E _;;
+        Ret (add Id v mem, MkStRef S (V Id) idx)
+      | ReadSTRef _ Id s =>
+        v <- lookup_err Id mem;;
+        Ret (mem, v)
+      | WriteSTRef _ Id s v =>
+        Ret (add Id v mem, tt)
+      end.
 
-End Translation.
+
 
 (* Example Programs*)
-Section ExampleTrees.
-
-  Context {S : Type}.
-  Context {E : Type -> Type}.
-  Context `{IdxGenE -< E}.
-  Context `{exceptE Err -< E}.
-
-
-  Definition E0 := STEvent S +' E.
-
-  Definition newAndReadBoth : itree E0 (nat * nat) :=
-    r1 <- newSTRef 5 ;;
-    r2 <- newSTRef 6 ;;
-    x1 <- readSTRef r1 ;;
-    x2 <- readSTRef r2 ;;
-    Ret (x1, x2).
-
-  Definition tree_simp : itree E0 nat :=
-    v <- newSTRef 5;;
-    readSTRef v.
-
-  (* NOTE: this failing definition is intentional, it should fail.
-    The intent is to test that we don't allow reference indices to escape. *)
-  Fail Definition tree_escape_example : itree E0 nat :=
-    v <- newSTRef 5;;
-    writeSTRef v (match v with mkSTRef _ _ idx => idx end);;
-    readSTRef v.
-
-  Definition tree_simp_another : itree E0 nat :=
-    v <- newSTRef 5;;
-    writeSTRef v 6;;
-    val <- readSTRef v;;
-    Ret val.
-
-
-End ExampleTrees.
 
 
 
 
-Section MemoryRep.
-
-Inductive node : Type := (* TODO: More types! *)
-  | NInt (x : nat) : node.
-
-
-Fixpoint node_to_type (n : node) : Type :=
-  match n with
-  | NInt x => nat
-  end.
-
-
-Class Convertible t := {
-    to_node : t -> node;
-    from_node: node -> option t;
-    node_convert_inverse: forall v : t, (from_node (to_node v)) = Some v
-  }.
-
-
-End MemoryRep.
 
 (* Interpretation in Rocq *)
-
-
-Section InterpST.
 
 
 
   (* TODO: better name perhaps *)
   Definition handle_STEvent_leave_rest
-    {S : Type}
-    {mem} `{Map (Idx S) nat mem}
-    {E : Type -> Type} `{exceptE Err -< E} `{IdxGenE -< E}
-    (T : Type) (e : (STEvent S +' E) T)
+    {mem} `{HMap (Idx S) V mem}
+    (T : Type) (e : (STEvent' S +' E) T)
     : stateT mem (itree (E)) T :=
     match e with
     | inl1 e0 => handle_STEvent T e0
-    | inr1 e0 => fun st : mem => r <- trigger e0;; ret (st, r)
+    | inr1 e0 => fun st : mem => r <- trigger e0;; Ret (st, r)
     end.
 
 
   Global Instance reldec_idx {S : Type} : @RelDec.RelDec (Idx S) eq :=
     (RelDec.RelDec_from_dec eq (IdxDecEq S)).
-    
-  Global Instance map_from_idx {S : Type} {V : Type}  : 
-    Map (Idx S) V (alist (Idx S) V) :=
-    Map_alist (RelDec.RelDec_from_dec eq (IdxDecEq S)) V.
 
-  Global Instance reldec_idx_correct {S : Type} : @RelDec.RelDec_Correct (Idx S) eq reldec_idx.
+  Global Instance hmap_from_idx :
+    HMap (Idx S) V (halist (Idx S) V) :=
+    @HMap_halist (Idx S) V eq_equivalence (IdxDecEq S).
+
+  Global Instance reldec_idx_correct : @RelDec.RelDec_Correct (Idx S) eq reldec_idx.
   econstructor.
   intuition.
-  destruct (IdxDecEq S x y); try assumption.
-  - unfold RelDec.rel_dec in H. cbn in H.
-    destruct IdxDecEq in H.
-    + contradiction.
-    + discriminate H.
-  - cbn.
-    specialize (@reldec_idx S) as reldec.
+  destruct (IdxDecEq S x y) eqn:Hdec.
+  - destruct IdxDecEq in Hdec; try assumption.
+  - specialize (@reldec_idx S) as reldec.
     specialize (IdxDecEq S x y) as dec.
     destruct dec.
-    + unfold RelDec.rel_dec. unfold reldec_idx. unfold RelDec.RelDec_from_dec.
-      destruct (IdxDecEq S x y).
-      * reflexivity.
-      * contradiction.
     + contradiction.
-    Qed.
-
-
-  Global Instance map_idx_correct {S V : Type} :
-    MapOk eq (@map_from_idx S V).
-  unfold map_from_idx.
-  eapply MapLaws_alist; typeclasses eauto.
+    + unfold RelDec.rel_dec in *. unfold reldec_idx in *. unfold RelDec.RelDec_from_dec in *.
+      destruct (IdxDecEq S x y); try assumption.
+      discriminate H2.
+  - unfold RelDec.rel_dec in *. unfold reldec_idx in *. unfold RelDec.RelDec_from_dec in *.
+    destruct (IdxDecEq S x y); try assumption.
+    + reflexivity.
+    + contradiction.
   Qed.
 
+
+  Global Instance map_idx_correct :
+    HMapOk hmap_from_idx := HMapOk_halist (Idx S) V.
+
+
   Definition interp_st
-    {E : Type -> Type} {S : Type}
-    `{exceptE Err -< E} `{IdxGenE -< E}
-    {mem} `{Map (Idx S) nat mem}
-    : itree (STEvent S +' E) ~> stateT mem (itree (E)) :=
+    {mem} `{HMap (Idx S) V mem}
+    : itree (STEvent' S +' E) ~> stateT mem (itree (E)) :=
     interp_state handle_STEvent_leave_rest.
 
   
-  (* TODO: cleanup! *)
-  (* TODO: refactor to use interp_map? *)
-  Definition runSt {A : Type} {E : Type -> Type}
-     `{exceptE Err -< E} `{IdxGenE -< E}
-    (f : forall (S : Type), itree ((STEvent S) +' E) A)
+End Translation.
+
+  Definition runSt {A : Type}
+  {E : Type -> Type}
+  {S : Type}
+  {V : (Idx S) -> Type}
+  `{@STEvent S V -< E} 
+  `{exceptE Err -< E}
+  `{IdxGenE -< E}
+    (f : forall (S : Type), itree ((@STEvent S V) +' E) A)
     : itree E A :=
-    fmap snd (interp_st _ (f unit) Maps.empty).
-
+    fmap snd (interp_st _ (f unit) HMap.empty).
   
-  
-
-End InterpST.
-
-
 
 Section InterpSTTheorems.
 
-  (* TODO: refactor to above. *)
-  Context {E : Type -> Type}. (* other events *)
-  Context {S : Type}. (* state thread *)
-  Context `{exceptE Err -< E}. (* runtime checks  *)
-  Context `{IdxGenE -< E}. (* index generating event *)
-  Context {R : Type}. (* values contained in the map,  TODO: expand from one value type. *)
+  Context {E : Type -> Type}.
+  Context {S : Type}.
+  Context {V : (Idx S) -> Type}.
+  Context `{@STEvent S V -< E}. 
+  Context `{exceptE Err -< E}.
+  Context `{IdxGenE -< E}.
 
-  Definition mem := alist (Idx S) nat. 
-  Global Instance mem_instance {V : Type} : 
-    Map (Idx S) V (alist (Idx S) V) :=
-    Map_alist (RelDec.RelDec_from_dec eq (IdxDecEq S)) V.
+  Definition mem := halist (Idx S) V.
 
+  Global Instance mem_instance : 
+    HMap (Idx S) V mem := @hmap_from_idx S V.
 
   Definition _interp_st {T : Type}
-    (ot : itree' (STEvent S +' E) T)
+    (ot : itree' (STEvent' S +' E) T)
     (l : mem)
     : itree E (mem * T) :=
     match ot with
@@ -370,7 +292,7 @@ Section InterpSTTheorems.
     end.
 
   Lemma unfold_interp_st {T : Type}
-    (t : itree (STEvent S +' E) T)
+    (t : itree (STEvent' S +' E) T)
     (l : mem) :
     eq_itree eq
     (interp_st _ t l)
@@ -390,28 +312,28 @@ Section InterpSTTheorems.
       reflexivity.
   Qed.
 
-  Lemma interp_st_ret: forall (val: R) (l : mem),
-      @interp_st E S _ _ _ _ _ (ret val) l ≅ ret (l, val).
+  Lemma interp_st_ret:  forall {R : Type} (val: R) (l : mem),
+      @interp_st E S _ _ _ _ _ _ (ret val) l ≅ ret (l, val).
     Proof using Type.
       intros. rewrite unfold_interp_st. reflexivity.
     Qed.
 
-  Lemma interp_st_Ret: forall (val: R) (l : mem),
-      @interp_st E S _ _ _ _ _ (Ret val) l ≅ Ret (l, val).
+  Lemma interp_st_Ret: forall {R : Type} (val: R) (l : mem),
+      @interp_st E S _ _ _ _ _ _ (Ret val) l ≅ Ret (l, val).
     Proof using Type.
       intros. rewrite unfold_interp_st. reflexivity.
     Qed.
 
   Lemma interp_st_Ret_eutt: forall {T : Type} (val: T) (l : mem),
-      @interp_st E S _ _ _ _ _ (Ret val) l ≈ Ret (l, val).
+      @interp_st E S _ _ _ _ _ _ (Ret val) l ≈ Ret (l, val).
     Proof using Type.
       intros. rewrite unfold_interp_st. reflexivity.
     Qed.
 
   Lemma interp_st_vis
     {T U} 
-    (e : (STEvent S +' E) T)
-    (k : T -> itree (STEvent S +' E) U)
+    (e : (STEvent' S +' E) T)
+    (k : T -> itree (STEvent' S +' E) U)
     (l : mem)
     : interp_st _ (Vis e k) l
     ≅ x <- handle_STEvent_leave_rest _ e l;;
@@ -422,7 +344,7 @@ Section InterpSTTheorems.
 
     
   Lemma interp_st_tau {T : Type}
-      (t : itree (STEvent S +' E) T)
+      (t : itree (STEvent' S +' E) T)
       (l : mem)
       : interp_st _ (Tau t) l ≅ Tau (interp_st _ t l).
     Proof using Type.
@@ -430,12 +352,12 @@ Section InterpSTTheorems.
     Qed.
 
 
-  Lemma Ret_is_ret (x : R) : ((Ret x) : itree E R)  = ret x.
+  Lemma Ret_is_ret {R : Type} (x : R) : ((Ret x) : itree E R)  = ret x.
     Proof using Type. reflexivity. Qed.
     
   Lemma interp_st_trigger
     {T : Type} 
-    (e : (STEvent S +' E) T)
+    (e : (STEvent' S +' E) T)
     (l : mem) :
     interp_st _ (ITree.trigger e) l ≈ handle_STEvent_leave_rest _ e l.
     Proof using Type.
@@ -457,25 +379,25 @@ Definition eq_itree_eqv_global {R E} (x1 x2 : itree (E) (mem * R)) : Prop :=
 
 
 Global Instance eq_itree_interp_st {T : Type} : 
-Proper (@eq_itree (STEvent S +' E) T T eq ==> eq ==> eq_itree_eqv_global)
+Proper (@eq_itree (STEvent' S +' E) T T eq ==> eq ==> eq_itree_eqv_global)
         (interp_st T).
 Proof using Type.
   repeat red.
   ginit. pcofix CIH. intros.
-  rewrite !unfold_interp_st. punfold H2. red in H2.
-    destruct H2; subst; pclearbot; try discriminate; cbn.
+  rewrite !unfold_interp_st. punfold H3. red in H3.
+    destruct H3; subst; pclearbot; try discriminate; cbn.
     - gstep; constructor; auto.
     - gstep; constructor; auto with paco.
     - guclo eqit_clo_bind. econstructor.
       + reflexivity.
-      + intros. gstep. rewrite H1. destruct u2 eqn:Equ2.
+      + intros. gstep. rewrite H2. destruct u2 eqn:Equ2.
         constructor; auto with paco itree.
   Qed.
 
     
-Lemma interp_st_bind {U} 
-  (t : itree (STEvent S +' E) R)
-  (k : R -> itree (STEvent S +' E) U)
+Lemma interp_st_bind {U R} 
+  (t : itree (STEvent' S +' E) R)
+  (k : R -> itree (STEvent' S +' E) U)
   (mem : mem)
   : interp_st U (ITree.bind t k) mem
       ≅ '(new_mem, new_val) <- interp_st R t mem;;
@@ -501,9 +423,9 @@ Lemma interp_st_bind {U}
       auto with paco.
 Qed.
 
-Lemma interp_st_bind_eutt {U} 
-  (t : itree (STEvent S +' E) R)
-  (k : R -> itree (STEvent S +' E) U)
+Lemma interp_st_bind_eutt {U R} 
+  (t : itree (STEvent' S +' E) R)
+  (k : R -> itree (STEvent' S +' E) U)
   (mem : mem)
   : interp_st U (ITree.bind t k) mem
       ≈ '(new_mem, new_val) <- interp_st R t mem;;
@@ -529,9 +451,9 @@ Lemma interp_st_bind_eutt {U}
       auto with paco.
 Qed.
 
-Lemma interp_st_bind_eutt' {U} 
-  (t : itree (STEvent S +' E) R)
-  (k : R -> itree (STEvent S +' E) U)
+Lemma interp_st_bind_eutt' {U R} 
+  (t : itree (STEvent' S +' E) R)
+  (k : R -> itree (STEvent' S +' E) U)
   (mem : mem)
   : (interp_st U (ITree.bind t k) mem)
       ≈ '(new_mem, new_val) <- interp_st R t mem;;
@@ -558,12 +480,12 @@ Lemma interp_st_bind_eutt' {U}
 Qed.
 
 
-Lemma eutt_eq_bind_interp_st {U}
+Lemma eutt_eq_bind_interp_st {U R}
   (k2 : (mem * R) -> itree E (mem * U))
   (lmem : mem)
-  (t1 : itree (STEvent S +' E) R)
+  (t1 : itree (STEvent' S +' E) R)
   (t2 : itree E (mem * R))
-  (k1: R -> itree (STEvent S +' E) U)
+  (k1: R -> itree (STEvent' S +' E) U)
   :
   interp_st R t1 lmem ≈ t2 ->
   (forall u lmem', interp_st U (k1 u) lmem' ≈ (k2 (lmem', u))) ->
@@ -586,239 +508,71 @@ Section STLookupErr.
   Context `{exceptE Err -< E}.
   Context {R : Type}.
   Context {map : Type}.
-  Context {Map : Map (Idx S) R map}.
-  Context {MOK : MapOk eq Map}.
+  Context {V : (Idx S) -> Type}.
 
-  Lemma st_lookup_err_add_eq : forall (s : map) (k : Idx S) (v : R),
-      lookup_err k (Maps.add k v s) = @ret (itree E) _ _ v.
+  (* Context {E : Type -> Type}.
+   * Context {S : Type}.
+   * Context {V : (Idx S) -> Type}.
+   * Context `{@STEvent S V -< E}. 
+   * Context `{exceptE Err -< E}.
+   * Context `{IdxGenE -< E}. *)
+
+  Context {hmap : HMap (Idx S) V map}.
+  Context {MOK : HMapOk hmap}.
+
+
+  (* TODO: generalize, move to utils/HMap. *)
+  Lemma st_lookup_add_eq : forall k v s, lookup k (add k v s) = Some v.
+    Proof.
+    intros.
+    rewrite mapsto_lookup; apply mapsto_add_eq. 
+    Unshelve. assumption.
+    Qed.
+
+  Lemma st_lookup_remove_eq :
+    forall k s, lookup k (HMap.remove k s) = None.
+  Proof using MOK.
+    intros.
+    destruct (lookup k (HMap.remove k s)) eqn:EQ.
+    - inversion MOK. 
+      rewrite mapsto_lookup in EQ.
+      exfalso.
+      eapply mapsto_remove_eq; eauto.
+    - reflexivity.
+    Qed.
+
+
+  
+  Lemma st_lookup_err_add_eq : forall (s : map) (k : Idx S) (v : (V k)),
+      lookup_err k (HMap.add k v s) = @ret (itree E) _ _ v.
   Proof using MOK.
     intros. unfold lookup_err.
-    rewrite (@lookup_add_eq (Idx S) R map Map MOK).
+    inversion MOK.
+    rewrite st_lookup_add_eq.
     reflexivity.
   Qed.
 
   Lemma st_lookup_err_remove_eq : forall (k : Idx S) (s : map),
-      lookup_err k (Maps.remove k s) = @throw Err E _ _ (Error "Failed to find key in map").
+      lookup_err k (HMap.remove k s) = @throw Err E _ _ (Error "Failed to find key in map").
   Proof using MOK.
     intros. unfold lookup_err.
-    rewrite (@lookup_remove_eq (Idx S) R map Map MOK k s).
+    rewrite st_lookup_remove_eq.
     reflexivity.
   Qed.
 
 End STLookupErr.
 
 
-
-Require Stdlib.derive.Derive.
-Section Examples.
-
-  Context {S : Type}.
-  Context {E : Type -> Type}.
-  Context `{IdxGenE -< E}.
-  Context `{exceptE Err -< E}.
-
-  Lemma eutt_fmap {E' : Type -> Type} {R U : Type} {t1 t2 : itree E' R} {f : R -> U} :
-    t1 ≈ t2 ->
-    fmap f t1 ≈ fmap f t2.
-    Proof using Type.
-      intros t_eq. apply eqit_map with (RR := eq).
-      + intros.
-        f_equal. assumption.
-      + apply t_eq.
-    Qed.
-
-       
-    
-  Lemma eutt_eq_bind {U R} (t : itree E U) (k1 k2: U -> itree E R):
-    (forall u, (k1 u) ≈ (k2 u)) ->
-    (ITree.bind t k1) ≈ (ITree.bind t k2).
-  Proof using Type. apply eutt_eq_bind. Qed.
-    
-
-  Lemma eutt_eq_bind' {U R}
-    (k1 k2: U -> itree E R)
-    (t1 t2: itree E U):
-    t1 ≈ t2 ->
-    (forall u, (k1 u) ≈ (k2 u)) ->
-    (ITree.bind t1 k1) ≈ (ITree.bind t2 k2).
-  Proof. apply eutt_eq_bind'. Qed.
-
-(* TODO: move to separate ltac section. *)
-Ltac refine_prod :=
-  (refine (fun '(a,b) => _)).
-
-Ltac refine_arg :=
-  (refine (fun arg => _)).
-
-Ltac refine_arg2 :=
-  (refine (fun arg1 arg2 => _)).
-
-
-
-Theorem bind_Ret_l : forall A B (f : A -> itree E B) (x : A), bind (Ret x) f ≈ f x.
-  setoid_rewrite Ret_is_ret.
-  setoid_rewrite Monad.bind_ret_l.
-  reflexivity.
-  Qed.
-          
-
-Theorem bind_Ret_r : forall A (x : itree E A), bind x (fun y => Ret y) ≈ x.
-  intros A x. setoid_rewrite Monad.bind_ret_r. reflexivity. Qed.
-
-
-Ltac monad_simpl_inner :=
-  repeat (repeat setoid_rewrite Monad.bind_bind;
-          repeat setoid_rewrite bind_Ret_l;
-          repeat setoid_rewrite bind_Ret_r).
-
-
-
-(* Useful for lifting ITree's back to a monad instance. *)
-Ltac change_to_monad :=
-  change (@ITree.bind ?E) with (@Monad.bind (itree E) _);
-  try setoid_rewrite Ret_is_ret.
-
-Ltac bind_split_refl_intros split_tactic :=
-  split_tactic ;[ reflexivity | intros]
-  ;cbv beta match.
-
-Opaque Maps.add.
-  
-  Derive (tree_simplified : itree E nat) in
-    ( runSt (fun S => @tree_simp S E)
-        ≈
-      tree_simplified
-    ) as tree_simplification.
-  Proof.
-    etransitivity.
-    { unfold runSt.
-      eapply eutt_fmap.
-      eapply (eutt_eq_bind_interp_st ltac:(refine_prod)).
-      - unfold newSTRef.
-        rewrite interp_st_trigger.
-        cbn.
-        reflexivity.
-      - intros u lmem'.
-        unfold readSTRef.
-        rewrite interp_st_trigger.
-        cbn.
-        reflexivity. }
-    etransitivity.
-    { eapply eutt_fmap.
-      change_to_monad.
-      monad_simpl_inner.
-      bind_split_refl_intros ltac:(eapply (eutt_eq_bind' _ ltac:(refine_arg))).
-      rewrite IdxRefSameIdx.
-      rewrite st_lookup_err_add_eq.
-      monad_simpl_inner.
-      reflexivity. }
-    cbn.
-    setoid_rewrite map_bind.
-    setoid_rewrite map_ret.
-    unfold snd.
-    unfold tree_simplified.
-    reflexivity.
-  Defined.
-
-
-  (* TODO: fill out the other examples in a likewise manner to above. *)
-  Derive (readboth_simplified : itree E (nat*nat)) in
-    ( runSt (fun S => @newAndReadBoth S E)
-        ≈
-      readboth_simplified
-    ) as tree_simplification2.
-  Proof.
-    etransitivity.
-    { unfold runSt.
-      eapply eutt_fmap.
-      eapply (eutt_eq_bind_interp_st ltac:(refine_arg)).
-      - unfold newSTRef.
-        rewrite interp_st_trigger.
-        cbn.
-        reflexivity.
-      - intros u lmem'.
-        unfold readSTRef.
-        eapply (eutt_eq_bind_interp_st ltac:(refine_arg)).
-        {
-          unfold newSTRef.
-          rewrite interp_st_trigger.
-          cbn.
-          change lmem' with (fst (lmem', u)). (* TODO: unfortunate change. *)
-          reflexivity.
-        }
-        intros ? ?.
-        eapply (eutt_eq_bind_interp_st ltac:(refine_arg)).
-        {
-          unfold newSTRef.
-          rewrite interp_st_trigger.
-          cbn. change u with (snd (lmem', u)).
-          change lmem'0 with (fst (lmem'0, u0)).
-          reflexivity.
-        }
-        intros ? ?. 
-        eapply (eutt_eq_bind_interp_st ltac:(refine_arg)).
-        {
-          unfold newSTRef.
-          rewrite interp_st_trigger.
-          cbn. change u with (snd (lmem', u)).
-          change lmem'0 with (fst (lmem'0, u0)).
-          change u0 with (snd (lmem'0, u0)).
-          change lmem'1 with (fst (lmem'1, u1)).
-          reflexivity.
-        }
-        intros ? ?.
-        rewrite interp_st_Ret.
-        change lmem'2 with (fst (lmem'2, u2)).
-        change u1 with (snd (lmem'1, u1)).
-        change u2 with (snd (lmem'2, u2)).
-        reflexivity. }
-    etransitivity.
-    { eapply eutt_fmap.
-      change_to_monad.
-      monad_simpl_inner.
-      bind_split_refl_intros ltac:(eapply (eutt_eq_bind' _ ltac:(refine_arg))).
-      monad_simpl_inner.
-      bind_split_refl_intros ltac:(eapply (eutt_eq_bind' _ ltac:(refine_arg))).
-      monad_simpl_inner. cbn.
-      rewrite IdxRefSameIdx.
-      Transparent Maps.add. unfold lookup_err at 1.
-      assert (lookup u (add u0 6 (add u 5 [])) = Some 5).
-      {
-        cbn. give_up. (* TODO: needs uniqueness of elements from stream. *)
-      }
-
-      setoid_rewrite H1.
-      monad_simpl_inner.
-      setoid_rewrite IdxRefSameIdx.
-      setoid_rewrite st_lookup_err_add_eq.
-      monad_simpl_inner.
-      reflexivity.
-    }
-    cbn.
-    setoid_rewrite map_bind.
-    setoid_rewrite map_bind.
-    setoid_rewrite map_ret.
-    unfold snd.
-    unfold readboth_simplified.
-    reflexivity.
-    Abort.
-
-End Examples.
-
 (* CPP Bindings *)
 
-  
-From Crane Require Extraction.
-
-
-(* TODO: how to obtain integer reference statically? *)
 Crane Extract Inlined Constant STRef => "%t1".
 Crane Extract Inlined Constant newSTRef => "%result = %a0".
 Crane Extract Inlined Constant readSTRef => "%a0". 
 Crane Extract Inlined Constant writeSTRef => "%a0 = %a1".
 Crane Extract Skip IdxRefSameIdx.
 Crane Extract Skip IdxRefSameRef.
-Crane Extract Skip E0.
 Crane Extract Skip newIdx.
 
+End ST_IMPL.
 
+Export ST_IMPL.
