tests/monadic/stmonad/STMonadtest.v
@@ -1,0 +1,106 @@
+
+From Crane Require Import Monads.STMonad.   
+
+From Stdlib Require Import
+  Arith.PeanoNat
+  Arith.Peano_dec
+  Init.Peano
+  List
+  Morphisms
+  RelationClasses
+  Relation_Definitions
+  Setoid
+  Strings.String
+.
+
+From Crane Require Import Monads.ITree.
+From ExtLib Require Import
+  Data.Bool
+  Data.List
+  Data.Map.FMapAList
+  Data.Monads.EitherMonad
+  Data.Pair
+  Data.String
+  Structures.Functor
+  Structures.Maps
+  Structures.Traversable
+.
+
+
+From ITree Require Import
+  Events.Exception
+  Events.FailFacts
+  Events.MapDefault
+  Events.MapDefaultFacts
+  Events.State
+  Events.StateFacts
+  ITree
+  ITreeFacts
+.
+
+Import Monads.
+Import ListNotations.
+Import ProperNotations.
+Local Open Scope monad_scope.
+Local Open Scope string_scope.
+Import ST_IMPL.
+
+
+
+Section ExampleTrees.
+
+  Context {S : Type}.
+  Context {E : Type -> Type}.
+  Context `{IdxGenE -< E}.
+  Context `{exceptE Err -< E}.
+
+
+  Definition V : Idx S -> Type := fun _ => nat.
+  Definition E0 := (STEvent S V) +' E.
+
+(* newSTRef :
+ * forall {E : Type -> Type} {S : Type} (V : Idx S -> Type),
+ * STEvent S V -< E -> forall I : Idx S, V I -> itree E (STRef S (V I)) *)
+  About readSTRef.
+(* readSTRef :
+ * forall {E : Type -> Type} {S : Type} (V : Idx S -> Type),
+ * STEvent S V -< E -> forall I : Idx S, STRef S (V I) -> itree E (V I) *)
+  (* TODO: tricky to state below! *)
+  Definition newAndReadBoth : itree E0 (nat * nat) :=
+    r1 <- newSTRef V _ 5 ;;
+    r2 <- newSTRef V _ 6 ;;
+    x1 <- readSTRef V _ r1 ;;
+    x2 <- readSTRef V _ r2 ;;
+    Ret (x1, x2).
+
+  Definition tree_simp : itree E0 nat :=
+    v <- newSTRef 5;;
+    readSTRef v.
+
+  (* NOTE: this failing definition is intentional.
+    The intent is to test that we don't allow reference indices to escape. *)
+  Fail Definition tree_escape_example : itree E0 nat :=
+    v <- newSTRef 5;;
+    writeSTRef v (match v with mkSTRef _ _ idx => idx end);;
+    readSTRef v.
+
+  Definition tree_simp_another : itree E0 nat :=
+    v <- newSTRef 5;;
+    writeSTRef v 6;;
+    val <- readSTRef v;;
+    Ret val.
+
+
+  (* "swap" function from "Lazy Functional State Threads", by John Launchbury and Simon L Peyton Jones. *)
+  Definition swap (v w : STRef S nat) : itree E0 unit :=
+    a <- readSTRef v;;
+    b <- readSTRef w;;
+    writeSTRef v b;;
+    writeSTRef w a.
+
+End ExampleTrees.
+
+
+From Crane Require Import Mapping.NatIntStd.   
+Crane Extract Skip E0.
+Crane Extraction "stmonad" newAndReadBoth tree_simp tree_simp_another.
